Bdd/Choice.lean
@@ -101,7 +101,7 @@ def choice_helper_spec {O : OBdd n m} (hr : O.Reduced) (hj : O.1.root = node j) 
       simp only [Fin.getElem_fin, Vector.getElem_set_self, ↓reduceIte]
       have : (O.high hj).evaluate ((choice_helper (O.high hj) hh (Vector.replicate n false)).set O.1.heap[j.1].var.1 true) =
              (O.high hj).evaluate (choice_helper (O.high hj) hh ((Vector.replicate n false))) := by
-        rw [Independence' (O.high hj) ⟨O.1.heap[j.1].var.1, ?_⟩ true (choice_helper (O.high hj) hh (Vector.replicate n false))]
+        rw [OBdd.independentOf_lt_root (O.high hj) ⟨O.1.heap[j.1].var.1, ?_⟩ true (choice_helper (O.high hj) hh (Vector.replicate n false))]
         rw [show O.1.heap[j.1].var.1 = O.var by simp [hj]]
         exact var_lt_high_var
       rw [this]
