Bdd/Sim.lean
@@ -8,15 +8,30 @@ namespace Sim
 structure State (O : OBdd n m) (U : OBdd n m') where
   lr : Std.HashMap (Fin m) (Fin m')
   rl : Std.HashMap (Fin m') (Fin m)
-  hl : ∀ j j', lr[j]? = some j' → rl[j']? = some j ∧ Pointer.Reachable O.1.heap O.1.root (.node j)  ∧ ∃ hj : Bdd.Ordered ⟨O.1.heap, .node j⟩, ∃ hj' : Bdd.Ordered ⟨U.1.heap, .node j'⟩, OBdd.HSimilar ⟨⟨O.1.heap, .node j⟩, hj⟩ ⟨⟨U.1.heap, .node j'⟩, hj'⟩
-  hr : ∀ j j', rl[j']? = some j → lr[j]? = some j' ∧ Pointer.Reachable U.1.heap U.1.root (.node j') ∧ ∃ hj : Bdd.Ordered ⟨O.1.heap, .node j⟩, ∃ hj' : Bdd.Ordered ⟨U.1.heap, .node j'⟩, OBdd.HSimilar ⟨⟨O.1.heap, .node j⟩, hj⟩ ⟨⟨U.1.heap, .node j'⟩, hj'⟩
+  hl : ∀ j j',
+    lr[j]? = some j' → rl[j']? = some j           ∧
+    Pointer.Reachable O.1.heap O.1.root (.node j) ∧
+    ∃ hj : Bdd.Ordered ⟨O.1.heap, .node j⟩,
+      ∃ hj' : Bdd.Ordered ⟨U.1.heap, .node j'⟩,
+        OBdd.HSimilar ⟨⟨O.1.heap, .node j⟩, hj⟩ ⟨⟨U.1.heap, .node j'⟩, hj'⟩
+  hr : ∀ j j',
+    rl[j']? = some j → lr[j]? = some j'            ∧
+    Pointer.Reachable U.1.heap U.1.root (.node j') ∧
+    ∃ hj : Bdd.Ordered ⟨O.1.heap, .node j⟩,
+      ∃ hj' : Bdd.Ordered ⟨U.1.heap, .node j'⟩,
+        OBdd.HSimilar ⟨⟨O.1.heap, .node j⟩, hj⟩ ⟨⟨U.1.heap, .node j'⟩, hj'⟩
 
 def sim_helper
     (O : OBdd n m) (hO : OBdd.Reduced O)
     (U : OBdd n m') (hU : OBdd.Reduced U)
     (p : Pointer m) (hpr : Pointer.Reachable O.1.heap O.1.root p)
     (q : Pointer m') (hqr : Pointer.Reachable U.1.heap U.1.root q) :
-  StateM (State O U) (Decidable (OBdd.HSimilar ⟨⟨O.1.heap, p⟩, Bdd.ordered_of_reachable hpr⟩ ⟨⟨U.1.heap, q⟩, Bdd.ordered_of_reachable hqr⟩)) := do
+  StateM
+    (State O U)
+    (Decidable
+      (OBdd.HSimilar
+        ⟨⟨O.1.heap, p⟩, Bdd.ordered_of_reachable hpr⟩
+        ⟨⟨U.1.heap, q⟩, Bdd.ordered_of_reachable hqr⟩)) := do
   match hp : p with
   | .terminal b =>
     match hq : q with
@@ -29,8 +44,8 @@ def sim_helper
     match hq : q with
     | .terminal b' => return isFalse (by simp [OBdd.HSimilar, OBdd.toTree_terminal', OBdd.toTree_node])
     | .node j' =>
-      match decEq O.1.heap[j].var U.1.heap[j'].var with
-      | isTrue hvt =>
+      if hv : O.1.heap[j].var = U.1.heap[j'].var
+      then
         let s ← get
         match hl : s.lr[j]? with
         | none =>
@@ -139,14 +154,10 @@ def sim_helper
               contradiction
             )
         | some i' =>
-          match decEq j' i' with
-          | isTrue heq =>
-            return isTrue (by
-              subst heq
-              rcases s.hl j j' hl with ⟨h1, h2, h3, h4, h5⟩
-              exact h5
-            )
-          | isFalse heq =>
+          if heq : j' = i'
+          then
+            return isTrue (s.hl j j' (by simp_all)).2.2.2.2
+          else
             return isFalse (fun c ↦ heq (by
               rcases s.hl j i' hl with ⟨h1, h2, h3, h4, h5⟩
               simp only [OBdd.HSimilar] at c h5
@@ -156,7 +167,7 @@ def sim_helper
               simp [InvImage] at this
               exact this
             ))
-      | isFalse hvf => return isFalse (fun c ↦ by simp [OBdd.HSimilar, OBdd.toTree_node] at c; exact hvf c.1)
+      else return isFalse (by simp_all [OBdd.HSimilar, OBdd.toTree_node])
 termination_by OBdd.size' (⟨⟨O.1.heap, p⟩, Bdd.ordered_of_reachable hpr⟩ : OBdd n m)
 decreasing_by
   · simp [OBdd.size_node, OBdd.low, Bdd.low]; omega
